src/simulation/SimRelationsHelpers.v
@@ -1,0 +1,46 @@
+From hahn Require Import Hahn.
+From imm Require Import CertCOhelper. 
+From imm Require Import Events.
+Require Import AuxRel.
+
+(* TODO: move the whole file contents to CombRelations in CertCOhelper *)
+
+Add Parametric Morphism : col0 with signature
+    eq ==> (@set_subset actid) ==> (@set_subset actid) ==> eq ==>
+       (@inclusion actid) as col0_mori.
+Proof using.
+  ins. unfold col0. rewrite H, H0. basic_solver. 
+Qed. 
+
+Add Parametric Morphism : col0 with signature
+    eq ==> (@set_equiv actid) ==> (@set_equiv actid) ==> eq ==>
+       (@same_relation actid) as col0_more.
+Proof using.
+  ins. destruct H, H0. 
+  split; apply col0_mori; basic_solver. 
+Qed.
+  
+Add Parametric Morphism : new_co with signature
+    eq ==> (@set_equiv actid) ==> (@set_equiv actid) ==>
+       (@inclusion actid) as new_co_more_impl.
+Proof using.
+  ins. unfold new_co, new_col.
+  unfolder. ins. desc. red in H1.
+  destruct H, H0.
+  exists l. des.
+  { left. eapply col0_mori; eauto. }
+  apply pref_union_alt.
+  right. split.
+  { splits; vauto.
+    { by apply H. }
+    intro. apply H6. basic_solver. }
+  intro. apply H4. eapply col0_mori; eauto. 
+Qed.  
+
+Add Parametric Morphism : new_co with signature
+    eq ==> (@set_equiv actid) ==> (@set_equiv actid) ==>
+       (@same_relation actid) as new_co_more.
+Proof using.
+  ins. split; [| symmetry in H, H0]; eapply new_co_more_impl; eauto.
+Qed. 
+
