src/tls_props/TlsAux.v
@@ -1,2 +1,0 @@
-Require Export TlsAux1.
-Require Export TlsAux2.
