src/tls_props/TlsEventSets.v
@@ -1,0 +1,281 @@
+From hahn Require Import Hahn.
+From imm Require Import TraversalOrder.
+From imm Require Import TLSCoherency.
+From imm Require Import IordCoherency.
+From imm Require Import Events.
+From imm Require Import Execution.
+Require Import AuxRel.
+From imm Require Import AuxDef.
+From imm Require Import imm_s.
+
+
+Definition covered  TLS := event ↑₁ (TLS ∩₁ action ↓₁ (eq ta_cover)).
+Definition issued   TLS := event ↑₁ (TLS ∩₁ action ↓₁ (eq ta_issue)).
+Definition reserved TLS := event ↑₁ (TLS ∩₁ action ↓₁ (eq ta_reserve)).
+Definition propagated G TLS :=
+  event ↑₁ (TLS ∩₁ (action ↓₁ is_ta_propagate_to_G G)). 
+
+
+Definition coverable G sc T :=
+  acts_set G ∩₁ event ↑₁ (dom_cond (iord G sc) T ∩₁ action ↓₁ eq ta_cover). 
+Definition issuable G sc T :=
+  acts_set G ∩₁ (is_w (lab G)) ∩₁ event ↑₁ (dom_cond (iord G sc) T ∩₁ action ↓₁ eq ta_issue). 
+
+
+Section MorphismsCIRP.
+
+Local Ltac cirp_morph :=
+  intros x y HH; unfold covered, issued, reserved, propagated;
+  solve [now rewrite HH|now rewrite <- HH].
+
+Global Add Parametric Morphism : covered with signature
+    (@set_subset trav_label) ==> (@set_subset actid)
+       as covered_mori.
+Proof using. cirp_morph. Qed.
+
+Global Add Parametric Morphism : issued with signature
+    (@set_subset trav_label) ==> (@set_subset actid)
+       as issued_mori.
+Proof using. cirp_morph. Qed.
+
+Global Add Parametric Morphism : reserved with signature
+    (@set_subset trav_label) ==> (@set_subset actid)
+       as reserved_mori.
+Proof using. cirp_morph. Qed.
+
+Global Add Parametric Morphism : propagated with signature
+    eq ==> (@set_subset trav_label) ==> (@set_subset actid)
+       as propagated_mori.
+Proof using. intros G. cirp_morph. Qed. 
+
+Global Add Parametric Morphism : covered with signature
+    (@set_equiv trav_label) ==> (@set_equiv actid)
+       as covered_more.
+Proof using. cirp_morph. Qed.
+
+Global Add Parametric Morphism : issued with signature
+    (@set_equiv trav_label) ==> (@set_equiv actid)
+       as issued_more.
+Proof using. cirp_morph. Qed. 
+
+Global Add Parametric Morphism : reserved with signature
+    (@set_equiv trav_label) ==> (@set_equiv actid)
+       as reserved_more.
+Proof using. cirp_morph. Qed. 
+
+Global Add Parametric Morphism : propagated with signature
+    eq ==> (@set_equiv trav_label) ==> (@set_equiv actid)
+       as propagated_more.
+Proof using. intros G. cirp_morph. Qed. 
+
+End MorphismsCIRP. 
+
+Section SimplificationsCIRP. 
+
+Lemma covered_events (A: actid -> Prop):
+  covered (event ↓₁ A) ⊆₁ A. 
+Proof using. unfold covered. basic_solver. Qed. 
+
+Lemma issued_events (A: actid -> Prop):
+  issued (event ↓₁ A) ⊆₁ A. 
+Proof using. unfold issued. basic_solver. Qed. 
+
+Lemma reserved_events (A: actid -> Prop):
+  reserved (event ↓₁ A) ⊆₁ A. 
+Proof using. unfold reserved. basic_solver. Qed. 
+
+Lemma propagated_events G (A: actid -> Prop):
+  propagated G (event ↓₁ A) ⊆₁ A. 
+Proof using. unfold propagated. basic_solver. Qed. 
+
+Lemma covered_union T1 T2:
+  covered (T1 ∪₁ T2) ≡₁ covered T1 ∪₁ covered T2. 
+Proof using. unfold covered. basic_solver 10. Qed. 
+
+Lemma issued_union T1 T2:
+  issued (T1 ∪₁ T2) ≡₁ issued T1 ∪₁ issued T2. 
+Proof using. unfold issued. basic_solver 10. Qed. 
+
+Lemma reserved_union T1 T2:
+  reserved (T1 ∪₁ T2) ≡₁ reserved T1 ∪₁ reserved T2. 
+Proof using. unfold reserved. basic_solver 10. Qed. 
+
+Lemma propagated_union G T1 T2:
+  propagated G (T1 ∪₁ T2) ≡₁ propagated G T1 ∪₁ propagated G T2. 
+Proof using. unfold propagated. basic_solver 10. Qed. 
+
+Lemma covered_singleton e:
+  covered (eq (mkTL ta_cover e)) ≡₁ eq e.
+Proof using. unfold covered. split; basic_solver. Qed. 
+
+Lemma issued_singleton e:
+  issued (eq (mkTL ta_issue e)) ≡₁ eq e.
+Proof using. unfold issued. split; basic_solver. Qed. 
+
+Lemma reserved_singleton e:
+  reserved (eq (mkTL ta_reserve e)) ≡₁ eq e.
+Proof using. unfold reserved. split; basic_solver. Qed. 
+
+(* TODO: find the correct statement and premises *)
+(* Lemma propagated_singleton G t e : *)
+(*   propagated G (eq (mkTL (ta_propagate t) e)) ≡₁ eq e. *)
+
+Lemma covered_noncover_empty S
+      (NONCOVER: set_disjoint S (action ↓₁ eq ta_cover)):
+  covered S ≡₁ ∅.
+Proof using. unfold covered. split; basic_solver. Qed. 
+
+Lemma issued_nonissue_empty S
+      (NONISSUE: set_disjoint S (action ↓₁ eq ta_issue)):
+  issued S ≡₁ ∅.
+Proof using. unfold issued. split; basic_solver. Qed. 
+
+Lemma reserved_nonreserve_empty S
+      (NONISSUE: set_disjoint S (action ↓₁ eq ta_reserve)):
+  reserved S ≡₁ ∅.
+Proof using. unfold reserved. split; basic_solver. Qed. 
+
+End SimplificationsCIRP. 
+
+
+(* The idea for these tactics is to try simplifying all appropriate terms once *)
+(* TODO: is there a better way to do this? *)
+Ltac remember_tls_sets :=
+  repeat (match goal with
+          |  |- context [ (covered ?S) ] => remember (@covered S) eqn:?HeqS
+          |  |- context [ (issued ?S) ] => remember (@issued S) eqn:?HeqS
+          |  |- context [ (reserved ?S) ] => remember (@reserved S) eqn:?HeqS
+          end).
+
+Ltac subst_tls_sets_simpl :=
+  repeat (match goal with
+          | H: ?E = covered ?S |- _ => subst E; try (rewrite covered_noncover_empty; [| basic_solver 10])
+          | H: ?E = issued ?S |- _ => subst E; try (rewrite issued_nonissue_empty; [| basic_solver 10])
+          | H: ?E = reserved ?S |- _ => subst E; try (rewrite reserved_nonreserve_empty; [| basic_solver 10])
+            end
+         ).
+
+Ltac simplify_tls_events :=
+  (repeat rewrite ?covered_union, ?issued_union, ?reserved_union);
+  (repeat rewrite ?covered_singleton, ?issued_singleton, ?reserved_singleton);
+  remember_tls_sets; subst_tls_sets_simpl. 
+
+
+Section WfSets.
+  Context (G: execution) (sc: relation actid) (WF: Wf G). 
+  Context
+    (T : trav_label -> Prop)
+    (TLSCOH  : tls_coherent G T)
+    (IORDCOH : iord_coherent G sc T).
+  
+  Notation "'E'" := (acts_set G).
+  Notation "'W'" := (fun x => is_true (is_w (lab G) x)).
+
+  Lemma issuedW :
+    issued T ⊆₁ W.
+  Proof using WF TLSCOH. 
+    unfold issued. rewrite tlsc_I_in_W; eauto. basic_solver.  
+  Qed. 
+
+  Lemma propagatedW : propagated G T ⊆₁ W.
+  Proof using WF TLSCOH.
+    clear -WF TLSCOH.
+    unfold propagated.
+    unfolder. ins. desf.
+    unfold is_ta_propagate_to_G in *.
+    unfolder in *. desf.
+    eapply tlsc_P_in_W; eauto.
+    basic_solver.
+  Qed. 
+
+  Lemma issuedE :
+    issued T ⊆₁ E.
+  Proof using WF TLSCOH.
+    unfold issued. rewrite (tlsc_E WF TLSCOH). basic_solver.  
+  Qed. 
+
+  Lemma coveredE:
+    covered T ⊆₁ E.
+  Proof using WF TLSCOH.
+    unfold covered. rewrite (tlsc_E WF TLSCOH). basic_solver.
+  Qed. 
+
+  Lemma w_covered_issued :
+    W ∩₁ covered T ⊆₁ issued T.
+  Proof using TLSCOH IORDCOH.
+    unfold covered.
+    unfolder. ins. desc.
+    forward eapply tlsc_w_covered_issued with (x := mkTL ta_cover x); eauto.
+    destruct y; ins; vauto. 
+  Qed.
+
+  Lemma init_issued : is_init ∩₁ E ⊆₁ issued T.
+  Proof using TLSCOH.
+    unfolder; ins; desf. red.
+    exists (mkTL ta_issue x). repeat split; auto. 
+    destruct TLSCOH. apply tls_coh_init. red. split; basic_solver. 
+  Qed. 
+
+  Lemma init_covered : is_init ∩₁ E ⊆₁ covered T.
+  Proof using TLSCOH. 
+    unfolder; ins; desf. red.
+    exists (mkTL ta_cover x). repeat split; auto. 
+    destruct TLSCOH. apply tls_coh_init. red. split; basic_solver. 
+  Qed.
+
+  Lemma covered_in_coverable: 
+    covered T ⊆₁ coverable G sc T.
+  Proof using WF TLSCOH IORDCOH. 
+    unfold covered, coverable. apply set_subset_inter_r. split; [apply coveredE|].
+    apply set_collect_mori; [done| ]. apply set_subset_inter; [| done].
+    by apply dom_rel_to_cond.
+  Qed.
+
+  Lemma issued_in_issuable:
+    issued T ⊆₁ issuable G sc T.
+  Proof using WF TLSCOH IORDCOH. 
+    unfold issued, issuable. repeat (apply set_subset_inter_r; split); auto using issuedE, issuedW. 
+    apply set_collect_mori; [done| ]. apply set_subset_inter; [| done].
+    by apply dom_rel_to_cond.
+  Qed.
+
+  Lemma w_coverable_issued :
+    W ∩₁ coverable G sc T ⊆₁ issued T.
+  Proof using TLSCOH.
+    rewrite AuxRel2.set_split_complete with (s' := _ ∩₁ _) (s := is_init).
+    apply set_subset_union_l. split.
+    { rewrite <- init_issued. unfold coverable. basic_solver. } 
+    rewrite <- dom_eqv with (d := _ ∩₁ _). rewrite id_inter, seq_eqvC. 
+    unfold coverable, issued. rewrite !id_inter, <- !seqA. 
+    eapply dom_rel_iord_ext_parts.
+    3: by apply init_issued.
+    2: basic_solver. 
+    transitivity (RF G); [| unfold iord_simpl; basic_solver 10].
+    unfold RF. hahn_frame. basic_solver 10. 
+  Qed.
+
+End WfSets. 
+
+(* TODO: move to IordCoherency in IMM *)
+Lemma iord_coherent_extend G sc T lbl
+      (ICOH: iord_coherent G sc T)
+      (ADD: dom_cond (iord G sc) T lbl):
+  iord_coherent G sc (T ∪₁ eq lbl). 
+Proof using. 
+  red. rewrite id_union, seq_union_r, dom_union.
+  red in ICOH, ADD. rewrite ICOH, ADD. basic_solver. 
+Qed.
+
+(* TODO: move to IordCoherency in IMM *)
+Lemma iord_coherent_element_prefix G sc (T: trav_label -> Prop) (lbl: trav_label)
+      (Tlbl: T lbl)
+      (ICOH: iord_coherent G sc T)
+      (IMMCON: imm_consistent G sc)
+      (WF: Wf G):
+  dom_rel (iord G sc ⨾ ⦗eq lbl⦘) ⊆₁ T \₁ eq lbl.
+Proof using.
+  rewrite set_minusE. apply set_subset_inter_r. split.
+  { etransitivity; [| apply ICOH]. basic_solver. }
+  intros x [y [REL ->]%seq_eqv_r]. intros ->.  
+  edestruct iord_irreflexive; eauto; apply IMMCON.
+Qed.
